decreasing_exponential_flow.v
@@ -1,0 +1,495 @@
+Require Import c_util.
+Require Import geometry.
+Require Import CRreal.
+Require Import CRexp.
+Require Import CRln.
+Require Import flow.
+Set Implicit Arguments.
+Open Local Scope CR_scope.
+
+Definition CRln' (x: CR) (H: CRpos x): CR :=
+  CRln x (CRpos_lt_0_rev H).
+
+Implicit Arguments CRln' [].
+
+Hint Resolve t8 CRpos_lt_0_rev exp_pos CRmult_lt_0 CRln_le.
+
+Lemma CRln_mult': forall a b (p: CRpos a) (q: CRpos b) (r: CRpos (a * b)),
+  CRln' (a * b) r == CRln' a p + CRln' b q.
+Proof. intros. apply CRln_mult. Qed.
+
+Lemma CRln'_opp_mult x y (P: CRpos (- (x * y))) (Q: CRpos (-x)) (R: CRpos y):
+  CRpos (- x * y) -> CRln' _ P == CRln' _ Q + CRln' _ R.
+Proof with auto.
+  intros.
+  apply CRln_opp_mult.
+  apply CRpos_lt_0_rev...
+Qed.
+
+Definition noneOr (X: Type) (P: X -> Set) (o: option X): Set :=
+  match o with
+  | None => True
+  | Some x => P x
+  end.
+
+Definition someAnd (X: Type) (P: X -> Set) (o: option X): Set :=
+  match o with
+  | None => False
+  | Some x => P x
+  end.
+
+Definition optPos: optCR -> Set := noneOr CRpos.
+Definition optNeg: optCR -> Set := noneOr CRneg.
+
+Definition optPos_le_trans (x: CR) (H: CRpos x) (y: optCR): OCRle (Some x, y) -> optPos y :=
+  match y with
+  | None => fun _ => I
+  | Some v => @CRpos_le_trans x H v
+  end.
+
+Definition optNeg_le_trans (x: CR) (H: CRneg x) (y: optCR): OCRle (y, Some x) -> optNeg y :=
+  match y with
+  | None => fun _ => I
+  | Some v => @CRneg_le_trans x H v
+  end.
+
+Lemma OCRle_None_right x: OCRle (x, None).
+Proof. destruct x; exact I. Qed.
+
+Definition raw (x: CR) (t: Time): CR := x * exp (-t).
+
+Lemma raw_pos x t: CRpos x -> CRpos (raw x t).
+Proof with auto. intros. apply CRpos_mult... apply exp_pos'. Defined.
+
+Lemma raw_neg x t: CRneg x -> CRneg (raw x t).
+Proof with auto.
+  intros.
+  unfold raw.
+  apply CRneg_opp.
+  apply CRpos_wd with (-x * exp (-t)).
+    symmetry. apply CRopp_mult_l.
+  apply CRpos_mult.
+    apply CRpos_opp...
+  apply exp_pos'.
+Defined.
+
+Lemma raw_pos_inv x t: CRpos (raw x t) -> CRpos x.
+Proof with auto.
+  intros.
+  unfold raw in H.
+  apply CRpos_mult_inv with (exp (-t)).
+    apply CRpos_nonNeg.
+    apply CRpos_lt_0.
+    apply exp_pos.
+  apply CRpos_lt_0...
+Defined.
+
+Lemma raw_neg_inv x t: CRneg (raw x t) -> CRneg x.
+Proof with auto.
+  intros.
+  apply CRneg_opp.
+  apply CRpos_mult_inv with (exp (-t))...
+    apply CRpos_nonNeg.
+    apply exp_pos'.
+  apply CRpos_wd with (-(x * exp (-t))).
+    apply CRopp_mult_l.
+  apply CRpos_opp...
+Defined.
+
+Lemma mono: forall x a b, CRpos x -> a < b -> raw x b < raw x a.
+Proof with auto.
+  repeat intro.
+  unfold raw.
+  apply CRmult_lt_pos_r...
+  apply exp_inc.
+  apply CRlt_opp_compat...
+Defined.
+
+Lemma raw_lt_compat_l: forall x a b, CRpos x -> a < b -> raw a x < raw b x.
+Proof with auto.
+  intros.
+  unfold raw.
+  apply CRlt_wd with (exp (-x) * a) (exp (-x) * b).
+      apply (Rmul_comm CR_ring_theory).
+    apply (Rmul_comm CR_ring_theory).
+  apply CRmult_lt_pos_r...
+  apply CRpos_lt_0.
+  apply exp_pos.
+Defined.
+
+Lemma raw_le_compat_l: forall x a b, a <= b -> raw a x <= raw b x.
+Proof with auto.
+  intros.
+  unfold raw.
+  rewrite (Rmul_comm CR_ring_theory a).
+  rewrite (Rmul_comm CR_ring_theory b).
+  apply CRmult_le_compat_r...
+  apply CRpos_nonNeg.
+  apply CRpos_lt_0.
+  apply exp_pos.
+Qed.
+
+Lemma raw_le_inv_r: forall x a b, CRnonNeg x -> raw x b <= raw x a -> a <= b.
+Proof with auto.
+  unfold raw.
+  intros.
+  apply CRle_opp_inv.
+  apply (exp_le_inv).
+  apply CRmult_le_inv with x...
+Qed.
+
+Definition morphism: binary_setoid_morphism CRasCSetoid CRasCSetoid CRasCSetoid.
+Proof.
+  apply (Build_binary_setoid_morphism _ _ _ raw).
+  intros. unfold raw.
+  rewrite H. rewrite H0. reflexivity.
+Defined.
+
+Lemma A x: x * exp (-'0) == x.
+  intros.
+  rewrite CRopp_0.
+  rewrite exp_0.
+  rewrite (Rmul_comm CR_ring_theory).
+  apply (Rmul_1_l CR_ring_theory).
+Qed.
+
+Lemma B x t t': x * exp (- (t + t'))[=]x * exp (- t) * exp (- t').
+  intros.
+  rewrite <- (Rmul_assoc CR_ring_theory).
+  rewrite <- exp_sum.
+  rewrite (@Ropp_add _ _ _ _ _ _ _ _ t3 CR_ring_eq_ext CR_ring_theory).
+  reflexivity.
+Qed.
+
+Definition f: Flow CRasCSetoid := Build_Flow morphism A B.
+
+Definition part_inv (x x': CR) (xp: CRpos x) (x'p: CRpos x'): Time := CRln' _ xp - CRln' _ x'p.
+
+Lemma part_inv_correct (x: CR) (xp: CRpos x) (x': CR) (x'p: CRpos x'):
+  raw x (part_inv xp x'p) == x'.
+Proof with auto.
+  unfold raw, part_inv.
+  intros.
+  rewrite <- diff_opp.
+  rewrite exp_sum.
+  unfold CRln'.
+  rewrite exp_ln.
+  rewrite (Rmul_comm CR_ring_theory x').
+  rewrite (Rmul_assoc CR_ring_theory).
+  rewrite exp_opp_ln.
+  apply (Rmul_1_l CR_ring_theory).
+Qed.
+
+Definition upper_shortest (src dst: OpenRange):
+  optPos (fst (`src)) -> optPos (snd (`dst)) -> optCR :=
+  match src, dst return optPos (fst (`src)) -> optPos (snd (`dst)) -> optCR with
+  | exist p _, exist q _ =>
+    match p, q return optPos (fst p) -> optPos (snd q) -> optCR with
+    | (x, _), (_, u) =>
+      match u, x return optPos x -> optPos u -> optCR with
+      | Some v, Some w =>
+        fun B E => Some (part_inv B E)
+      | _, _ => fun _ _ => None
+  end end end.
+
+Definition upper_longest (src dst: OpenRange):
+  optPos (snd (`src)) -> optPos (fst (`dst)) -> optCR :=
+  match src, dst return optPos (snd (`src)) -> optPos (fst (`dst)) -> optCR with
+  | exist p _, exist q _ =>
+    match p, q return optPos (snd p) -> optPos (fst q) -> optCR with
+    | (_, x), (u, _) =>
+      match u, x return optPos x -> optPos u -> optCR with
+      | Some v, Some w =>
+        fun B E => Some (part_inv B E)
+      | _, _ => fun _ _ => None
+  end end end.
+
+Definition lower_shortest (src dst: OpenRange):
+  optNeg (snd (`src)) -> optNeg (fst (`dst)) -> optCR :=
+  match src, dst return optNeg (snd (`src)) -> optNeg (fst (`dst)) -> optCR with
+  | exist p _, exist q _ =>
+    match p, q return optNeg (snd p) -> optNeg (fst q) -> optCR with
+    | (_, x), (u, _) =>
+      match u, x return optNeg x -> optNeg u -> optCR with
+      | Some v, Some w =>
+        fun B E => Some (part_inv (CRpos_opp B) (CRpos_opp E))
+      | _, _ => fun _ _ => None
+  end end end.
+
+Definition lower_longest (src dst: OpenRange):
+  optNeg (fst (`src)) -> optNeg (snd (`dst)) -> optCR :=
+  match src, dst return optNeg (fst (`src)) -> optNeg (snd (`dst)) -> optCR with
+  | exist p _, exist q _ =>
+    match p, q return optNeg (fst p) -> optNeg (snd q) -> optCR with
+    | (x, _), (_, u) =>
+      match u, x return optNeg x -> optNeg u -> optCR with
+      | Some v, Some w =>
+        fun B E => Some (part_inv (CRpos_opp B) (CRpos_opp E))
+      | _, _ => fun _ _ => None
+  end end end.
+
+      (* i have some faith that some of these return clauses can be omitted in a future Coq version *)
+
+Section upper_def.
+
+  Variable (src dst: OpenRange)
+    (src_fst_nonNeg: optPos (fst (`src)))
+    (src_snd_nonNeg: optPos (snd (`src)))
+    (dst_fst_nonNeg: optPos (fst (`dst)))
+    (dst_snd_nonNeg: optPos (snd (`dst))).
+
+  Program Definition upper: OpenRange :=
+    (upper_shortest src dst src_fst_nonNeg dst_snd_nonNeg
+    , upper_longest src dst src_snd_nonNeg dst_fst_nonNeg).
+  Next Obligation. Proof with auto.
+    destruct src. destruct dst.
+    simpl.
+    destruct x. destruct x0.
+    destruct s2...
+    destruct s...
+    destruct s1...
+    destruct s0...
+    unfold part_inv.
+    unfold CRln'.
+    apply t9...
+  Defined.
+
+  Variables
+    (x: CR) (xnn: CRnonNeg x)
+    (xisrc: in_orange src x)
+    (t: Time) (xidst: in_orange dst (raw x t)).
+
+  Lemma part_inv_alt (H3: CRpos x) (H4 : CRpos (raw x t)): t[=]part_inv H3 H4.
+  Proof with auto.
+    intros. unfold part_inv, raw.
+    assert (CRpos (exp (-t))) by apply exp_pos'.
+    rewrite (CRln_mult' H3 H H4).
+    unfold CRln'.
+    rewrite CRln_exp.
+    rewrite <- diff_opp.
+    rewrite <- t11.
+    reflexivity.
+  Qed.
+
+  Lemma upper_correct: in_orange upper t.
+  Proof with auto.
+    unfold upper, in_orange, orange_left, orange_right.
+    simpl. destruct src. destruct dst. destruct x0. destruct x1.
+    simpl. split.
+      destruct s2... destruct s... destruct xisrc. destruct xidst.
+      simpl in H, H2, src_fst_nonNeg, src_snd_nonNeg, dst_fst_nonNeg, dst_snd_nonNeg.
+      assert (CRpos x). apply CRpos_le_trans with s...
+      rewrite (part_inv_alt H3 (raw_pos t H3)).
+      unfold part_inv.
+      apply t9; unfold CRln'...
+    destruct s1... destruct s0... destruct xisrc. destruct xidst.
+    simpl in H0, H1, src_fst_nonNeg, src_snd_nonNeg, dst_fst_nonNeg, dst_snd_nonNeg.
+    assert (CRpos (raw x t)). apply CRpos_le_trans with s1...
+    rewrite (part_inv_alt (raw_pos_inv H3) H3).
+    apply t9; unfold CRln'...
+  Qed.
+
+End upper_def.
+
+Section lower_def.
+
+  Variables (src dst: OpenRange)
+    (src_fst_nonPos: optNeg (fst (`src)))
+    (src_snd_nonPos: optNeg (snd (`src)))
+    (dst_fst_nonPos: optNeg (fst (`dst)))
+    (dst_snd_nonPos: optNeg (snd (`dst))).
+
+  Program Definition lower: OpenRange :=
+    (lower_shortest src dst src_snd_nonPos dst_fst_nonPos
+    , lower_longest src dst src_fst_nonPos dst_snd_nonPos).
+  Next Obligation. Proof with auto.
+    destruct src. destruct dst.
+    destruct x. destruct x0.
+    simpl.
+    destruct s1...
+    destruct s0...
+    destruct s2...
+    destruct s...
+    unfold part_inv.
+    apply t9; unfold CRln'...
+  Defined.
+
+  Variables
+    (x: CR) (xnn: CRnonNeg x)
+    (xisrc: in_orange src x)
+    (t: Time) (xidst: in_orange dst (raw x t)).
+
+  Lemma lower_part_inv_alt (H3: CRneg x) (H4: CRneg (raw x t)): t[=]part_inv (CRpos_opp H3) (CRpos_opp H4).
+  Proof with auto.
+    intros. unfold part_inv, raw.
+    rewrite (CRln'_opp_mult (CRpos_opp H4) (CRpos_opp H3) (exp_pos' (-t))).
+      unfold CRln'.
+      rewrite CRln_exp.
+      rewrite <- diff_opp.
+      rewrite <- t11...
+    apply CRpos_wd with (- (x * exp (-t))).
+      apply CRopp_mult_l.
+    apply CRpos_opp...
+  Qed.
+
+  Lemma lower_correct: in_orange lower t.
+  Proof with auto.
+    unfold lower, in_orange, orange_left, orange_right.
+    simpl. destruct src. destruct dst. destruct x0. destruct x1.
+    simpl. split.
+      destruct s1... destruct s0... destruct xisrc. destruct xidst.
+      simpl in H0, H1, src_fst_nonPos, src_snd_nonPos, dst_fst_nonPos, dst_snd_nonPos.
+      assert (CRneg x). apply CRneg_le_trans with s0...
+      assert (CRneg (raw x t)). apply raw_neg...
+      rewrite (lower_part_inv_alt H3 H4).
+      apply t9; unfold CRln'...
+    destruct s2... destruct s... destruct xisrc. destruct xidst.
+    simpl in H, H2, src_fst_nonPos, src_snd_nonPos, dst_fst_nonPos, dst_snd_nonPos.
+    assert (CRneg (raw x t)). apply CRneg_le_trans with s2...
+    assert (CRneg x). apply raw_neg_inv with t...
+    rewrite (lower_part_inv_alt H4 H3).
+    unfold part_inv.
+    apply t9; unfold CRln'...
+  Qed.
+
+End lower_def.
+
+Definition someAnd_noneOr (X: Type) (P: X -> Set) (r: option X): someAnd P r -> noneOr P r :=
+  match r return someAnd P r -> noneOr P r with
+  | None => fun _ => I
+  | Some v => fun H => H
+  end.
+
+Definition upper_pos_from_lower (r: OpenRange):
+  someAnd CRpos (fst (`r)) -> optPos (snd (`r)).
+Proof.
+  intros [[[x|] y] le]; intros.
+    apply optPos_le_trans with x; assumption.
+  elimtype False. assumption.
+Defined.
+
+Definition lower_neg_from_upper (r: OpenRange):
+  someAnd CRneg (snd (`r)) -> optNeg (fst (`r)).
+Proof.
+  intros [[x [y|]] le]; intros.
+    apply optNeg_le_trans with y; assumption.
+  elimtype False. assumption.
+Defined.
+
+Section contents.
+
+  Variable (eps: Qpos).
+
+  Definition range_cases (r: OpenRange): option (
+    someAnd CRpos (fst (`r)) +
+    someAnd CRneg (snd (`r)) +
+    (optNeg (fst (`r)) * optPos (snd (`r)))) :=
+    match r return option (someAnd CRpos (fst (`r)) + someAnd CRneg (snd (`r)) + (optNeg (fst (`r)) * optPos (snd (`r)))) with
+    | exist p _ => match p return option (someAnd CRpos (fst p) + someAnd CRneg (snd p) + (optNeg (fst p) * optPos (snd p))) with
+      | (s, s0) => match s return option (someAnd CRpos s + someAnd CRneg s0 + (optNeg s * optPos s0)) with
+        | Some v => match CR_sign_dec eps v with
+          | None => None
+          | Some (inl U) => Some (inl (inl U))
+          | Some (inr U) => match s0 with
+            | None => Some (inr (pair U I))
+            | Some w => match CR_sign_dec eps w with
+              | Some (inl V) => Some (inr (pair U V))
+              | Some (inr V) => Some (inl (inr V))
+              | None => None
+          end end end
+        | None => match s0 with
+          | Some v => match CR_sign_dec eps v with
+            | Some (inl U) => Some (inr (pair I U))
+            | Some (inr U) => Some (inl (inr U))
+            | None => None
+            end
+          | None_ => Some (inr (pair I I))
+    end end end end.
+
+  Program Definition no_trans_result: OpenRange := (-'1, -'1): Range.
+
+  Definition inv (src dst: OpenRange): OpenRange.
+  Proof with auto.
+    intros.
+    refine (match range_cases src, range_cases dst with
+    | Some (inr _), Some (inr _) => unbounded_range
+    | Some (inr (pair U W)), Some (inl (inr V)) => _
+    | Some (inr (pair U W)), Some (inl (inl V)) => _
+    | Some (inl (inr U)), Some (inr (pair V W)) => _
+    | Some (inl (inr y)), Some (inl (inr y0)) => lower src dst (lower_neg_from_upper _ y) (someAnd_noneOr _ _ y) (lower_neg_from_upper _ y0) (someAnd_noneOr _ _ y0)
+    | Some (inl (inr _)), Some (inl (inl _)) => no_trans_result
+    | Some (inl (inl U)), Some (inr (pair V W)) => _
+    | Some (inl (inl _)), Some (inl (inr _)) => no_trans_result
+    | Some (inl (inl y)), Some (inl (inl y0)) => upper src dst (someAnd_noneOr _ _ y) (upper_pos_from_lower _ y) (someAnd_noneOr _ _ y0) (upper_pos_from_lower _ y0)
+    | None, _ => unbounded_range
+    | _, None => unbounded_range
+    end); try clear s; try clear s0; try clear s1; try clear s2; try destruct p;
+      destruct src; destruct dst; destruct x; destruct x0.
+          try (destruct s; [idtac | elimtype False; assumption]).
+          apply (upper (exist OCRle (Some s, s0) o1) (exist OCRle (None, s2) I) y)...
+            apply optPos_le_trans with s...
+          simpl...
+        (* src neg, dst has 0 *)
+        try (destruct s0; [idtac | elimtype False; assumption]).
+        apply (lower (exist OCRle (s, Some s0) o1) (exist OCRle (s1, None) (OCRle_None_right _))); simpl...
+        apply optNeg_le_trans with s0...
+      (* src has 0, dst pos *)
+      try (destruct s1; [idtac | elimtype False; assumption]).
+      apply (@upper (exist OCRle (None, s0) I) (exist OCRle (Some s1, s2) o2)); simpl...
+      apply optPos_le_trans with s1...
+    (* src has 0, dst neg *)
+    try (destruct s2; [idtac | elimtype False; assumption]).
+    apply (lower (exist OCRle (s, None) (OCRle_None_right s)) (exist OCRle (s1, Some s2) o2)); simpl...
+    apply optNeg_le_trans with s2...
+  Defined.
+
+  Lemma inv_correct: range_flow_inv_spec f inv.
+  Proof with auto.
+    unfold range_flow_inv_spec.
+    intros src x H dst t H0.
+    unfold inv.
+    destruct (range_cases src) as [[[P | Q] | R] | S];
+    destruct (range_cases dst) as [[[V | W] | X] | Y];
+      destruct src; destruct dst; destruct x0; destruct x1;
+      try (destruct s; [idtac | elimtype False; assumption]);
+      try (destruct s0; [idtac | elimtype False; assumption]);
+      try (destruct s1; [idtac | elimtype False; assumption]);
+      try (destruct s2; [idtac | elimtype False; assumption]); simpl...
+                      apply upper_correct with x...
+                    elimtype False.
+                    destruct H. destruct H0.
+                    simpl in H1, W, H, H2.
+                    apply CRneg_pos_excl with (raw x t).
+                      apply raw_pos...
+                      apply CRpos_lt_0.
+                      apply CRlt_le_trans with s...
+                    apply CRneg_le_trans with s2...
+                  destruct X.
+                  apply upper_correct with x...
+                  split; simpl...
+                  destruct H0...
+                elimtype False.
+                destruct H. destruct H0.
+                simpl in V, Q, H, H1, H0.
+                apply CRneg_pos_excl with (raw x t).
+                  apply CRpos_le_trans with s1...
+                apply raw_neg.
+                apply CRneg_le_trans with s0...
+              apply lower_correct with x...
+            destruct X.
+            apply lower_correct with x...
+            split; simpl...
+            destruct H0...
+          destruct R.
+          apply upper_correct with x...
+          split; simpl...
+          destruct H...
+        destruct R.
+        apply lower_correct with x...
+        split; simpl...
+        destruct H...
+      destruct R...
+    destruct R...
+  Qed.
+
+End contents.
